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Let p be a prime number. Given a nonzero integer n, we define the p-adic valuation vp(n) of
n to be the largest integer k such that pk | n.

More generally, given a nonzero rational number
m
n

where gcd(m, n) = 1, we define its p-

adic valuation vp

(m
n

)
as vp(m)− vp(n). However, we will assume the domain of vp is N

unless stated otherwise.

A few trivial facts:

• vp(mn) = vp(m) + vp(n). (They operate like logarithms)

• vp(n) = 0 if and only if p - n.

• vp(n) = k if and only if pk | n and pk+1 - n. We write this also as pk||n.

• vp(a + b) ≥ min(vp(a), vp(b)). (When is the equality strict?)

• (a + bp)k ≡ ak + kak−1bp (mod p2).

1 Warm Up

1. Denote sp(n) as the sum of digits of n in base p.

vp(n!) = ∑
k≥1

⌊
n
pk

⌋
=

n− sp(n)
p− 1

2. Prove that p does not divide
(

pkm
pk

)
where p - m.

3. Let a and b be integers such that a | b2, b3 | a4, a5 | b6, b7 | a8, · · · . Prove that a = b.

4. Prove that for all positive integers a, b, c,

lcm(a, b, c)2

lcm(a, b) · lcm(b, c) · lcm(c, a)
=

gcd(a, b, c)2

gcd(a, b) · gcd(b, c) · gcd(c, a)



2 Lifting the Exponent Lemma

We will analyse what vp(xn − yn) is in terms of x − y and n. Turns out that for suitable
conditions for x, y, the relation is simple. However, we need to separate into two regimes:

2.1 p 6= 2

Theorem 1. Assume x ≡ y 6≡ 0 (mod p). Then for any positive integer n,

vp(xn − yn) = vp(x− y) + vp(n).

Proof. We use induction, but first let’s settle a large number of cases: If p - n, then

xn − yn

x− y
=

n−1

∑
k=0

xn−1−kyk ≡
n−1

∑
k=0

xn−1−kxk ≡ nxn−1 6≡ 0 (mod p)

thus vp(xn − yn) = vp(x− y). Next, we prove that vp(xp − yp) = vp(x− y) + 1. To do this,
we prove that vp((xp − yp)/(x− y)) = 1. By taking mod p2 and letting y = x + pN,

xp − yp

x− y
=

p−1

∑
k=0

xp−1−k(x + Np)k

≡
p−1

∑
k=0

xp−1−k(xk + kxk−1Np)

≡
p−1

∑
k=0

(xp−1 + Npkxp−2)

≡ pxp−1 + Np · p(p− 1)
2

· xp−2

≡ pxp−1 (mod p2)

and hence this is divisible by p but not p2 (Where did we use p 6= 2?). Finish the proof. �

Theorem 2. Assume x ≡ −y 6≡ 0 (mod p). Then for any odd positive integer n,

vp(xn + yn) = vp(x + y) + vp(n).

Proof. Analogous to Theorem 1.



2.2 p = 2

Theorem 3. Assume x ≡ y 6≡ 0 (mod 2). Then for any odd positive integer n,

v2(xn ± yn) = v2(x± y).

Proof. Analogous to the first part of Theorem 1.

Theorem 4. Assume x ≡ y 6≡ 0 (mod 2). Then for any even positive integer n,

v2(xn − yn) = v2(x− y) + v2(x + y) + v2(n)− 1.

Proof. It suffices to prove for n = 2m (Why?):

v2

(
x2m − y2m

)
= v2

(
(x− y)

m−1

∏
k=0

(
x2k

+ y2k
))

= v2(x− y) + v2(x + y) +
m−1

∑
k=1

v2

(
x2k

+ y2k
)

= v2(x− y) + v2(x + y) +
m−1

∑
k=1

1 (Why?)

= v2(x− y) + v2(x + y) + m− 1. �

2.3 Exercises

1. Let k > 0 be fixed. Find all n ∈N such that 3k | 2n − 1.

2. Prove that if p is an odd prime, ap ≡ 1 (mod pn)⇒ a ≡ 1 (mod pn−1).

3. Find all x ∈N such that 4(xn + 1) is a perfect cube for all n > 0.

4. Let k > 1 be fixed. Show there are infinitely many n such that

n | 1n + 2n + · · ·+ kn.

5. Find all triples (a, b, p) of positive integers with p prime and

ap = b! + p.
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